txn-data-consistency/EP+_TCCv_Proof.thy
@@ -242,7 +242,7 @@ lemma pending_wtxns_adding_lb:
   using assms by (auto simp add: finite_nat_set_iff_bounded_le pending_wtxns_ts_def)
 
 lemma pending_wtxns_removing_lb:
-  assumes "\<forall>ts \<in> pending_wtxns_ts (svr_state (svrs s k)). ts \<ge> clk"
+  assumes "\<forall> ts \<in> pending_wtxns_ts (svr_state (svrs s k)). ts \<ge> clk"
   shows "\<forall>ts \<in> pending_wtxns_ts ((svr_state (svrs s k)) (Tn t := Commit cts sts lst v rs)). ts \<ge> clk"
   using assms by (auto simp add: finite_nat_set_iff_bounded_le pending_wtxns_ts_def)
 
@@ -400,17 +400,17 @@ next
   case (reach_trans s e s')
   then show ?case
   proof (induction e)
-    case (RegR x1 x2 x3 x4 x5)
+    case (RegR x1 x2 x3 x4 x5 x6 x7)
     then show ?case
       apply (auto simp add: Pend_Wt_UB_def tps_trans_defs pending_wtxns_ts_def)
       by (meson add_to_readerset_prep_inv le_SucI le_trans max.cobounded1)
   next
-    case (PrepW x1 x2 x3 x4)
+    case (PrepW x1 x2 x3 x4 x5)
     then show ?case
       apply (auto simp add: Pend_Wt_UB_def tps_trans_defs pending_wtxns_ts_def)
       by (meson le_Suc_eq max.coboundedI1)
   next
-    case (CommitW x1 x2 x3 x4 x5)
+    case (CommitW x1 x2 x3 x4 x5 x6 x7)
     then show ?case
       apply (auto simp add: Pend_Wt_UB_def tps_trans_defs pending_wtxns_ts_def split: if_split_asm)
       by (meson le_Suc_eq max.coboundedI1 notin_set_remove1)
@@ -433,15 +433,15 @@ next
   case (reach_trans s e s')
   then show ?case 
   proof (induction e)
-    case (RegR x71 x72 x73 x74)
+    case (RegR x71 x72 x73 x74 x75 x76 x77)
     then show ?case
       by (auto simp add: Finite_Pend_Inv_def tps_trans_defs finite_pending_wtxns_rtxn)
   next
-    case (PrepW x81 x82 x83)
+    case (PrepW x81 x82 x83 x84 x85)
     then show ?case
       by (auto simp add: Finite_Pend_Inv_def tps_trans_defs finite_pending_wtxns_adding)
   next
-    case (CommitW x91 x92)
+    case (CommitW x91 x92 x93 x94 x95 x96 x97)
     then show ?case
       by (auto simp add: Finite_Pend_Inv_def tps_trans_defs finite_pending_wtxns_removing)
   qed (auto simp add: Finite_Pend_Inv_def tps_trans_defs)
@@ -463,7 +463,7 @@ next
   case (reach_trans s e s')
   then show ?case 
   proof (induction e)
-    case (CommitW x91 x92 x93 x94 x95)
+    case (CommitW x91 x92 x93 x94 x95 x96 x97)
     then show ?case
       apply (auto simp add: Svr_Clk_le_Lst_def tps_trans_defs split: if_split_asm)
       by (smt Finite_Pend_Inv_def Min_le_iff Pend_Wt_UB_def emptyE finite_pending_wtxns_removing
@@ -486,23 +486,17 @@ next
   case (reach_trans s e s')
   then show ?case 
   proof (induction e)
-    case (RegR x1 x2 x3 x4 x5)
+    case (RegR x1 x2 x3 x4 x5 x6 x7)
     then show ?case by (auto simp add: Pend_Wt_LB_def tps_trans_defs pending_wtxns_rtxn)
   next
-    case (PrepW x1 x2 x3 x4)
+    case (PrepW x1 x2 x3 x4 x5)
     then show ?case apply (auto simp add: Pend_Wt_LB_def tps_trans_defs pending_wtxns_adding)
       by (metis Svr_Clk_le_Lst_def le_Suc_eq le_trans max.cobounded2 max.commute
           reach_svr_clock_svr_lst_inv reach_trans.hyps(2))
   next
-    case (CommitW x1 x2 x3 x4 x5)
+    case (CommitW x1 x2 x3 x4 x5 x6 x7)
     then show ?case apply (auto simp add: Pend_Wt_LB_def tps_trans_defs split: if_split_asm)
-      using Finite_Pend_Inv_def[of s]
-        pending_wtxns_removing_lb[of s x1 "svr_lst (svrs s x1)" x2 x4 "Suc (max (svr_clock (svrs s x1)) (cl_clock (cls s (get_cl x2))))" "svr_clock (svrs s x1)" x3 rs_emp]
-        finite_pending_wtxns_removing[of s x1 x2 x4 "Suc (max (svr_clock (svrs s x1)) (cl_clock (cls s (get_cl x2))))" "svr_clock (svrs s x1)" x3 rs_emp]
-       apply auto
-      subgoal sorry
-      subgoal (* apply (meson Finite_Pend_Inv_def Min_le finite_pending_wtxns_removing reach_finitepending)*) sorry
-      done
+      by (metis Finite_Pend_Inv_def Min.coboundedI finite_pending_wtxns_removing reach_finitepending)
   qed(auto simp add: Pend_Wt_LB_def tps_trans_defs)
 qed
 
@@ -515,19 +509,21 @@ lemma min_pending_wtxns_monotonic:
          Min (pending_wtxns_ts (svr_state (svrs s' k)))"
   using assms
 proof (induction e)
-  case (RegR x1 x2 x3 x4 x5)
+  case (RegR x1 x2 x3 x4 x5 x6 x7)
   then show ?case
   apply (auto simp add: tps_trans_defs pending_wtxns_ts_def)
     by (smt (z3) Collect_cong add_to_readerset_prep_inv nat_le_linear)
 next
-  case (PrepW x1 x2 x3 x4)
+  case (PrepW x1 x2 x3 x4 x5)
   then show ?case apply (auto simp add: tps_trans_defs)
     using Min_insert_larger[of "pending_wtxns_ts (svr_state (svrs s x1))"
-        "pending_wtxns_ts (svr_state (svrs s' x1))" "svr_clock (svrs s x1)"]
-      pending_wtxns_adding [of s x1] Pend_Wt_UB_def[of s] Finite_Pend_Inv_def[of s]
-    by (cases "k = x1"; auto simp add: pending_wtxns_ts_def)
+        "pending_wtxns_ts (svr_state (svrs s' x1))"
+        "(Suc (max (svr_clock (svrs s x1)) (cl_clock (cls s (get_cl x2)))))"]
+      pending_wtxns_adding [of s] Pend_Wt_UB_def[of s] Finite_Pend_Inv_def[of s]
+    apply (cases "k = x1"; auto simp add: pending_wtxns_ts_def)
+    by (meson le_SucI le_trans max.cobounded1)
 next
-  case (CommitW x1 x2 x3 x4 x5)
+  case (CommitW x1 x2 x3 x4 x5 x6 x7)
   then show ?case using Finite_Pend_Inv_def[of s]
     apply (auto simp add: tps_trans_defs fold_pending_wtxns_fun_upd)
     by (metis Min.coboundedI Min_in Min_remove empty_iff pending_wtxns_removing)
@@ -540,16 +536,17 @@ lemma svr_lst_monotonic:
   shows "svr_lst (svrs s' svr) \<ge> svr_lst (svrs s svr)"
   using assms
   proof (induction e)
-    case (CommitW k t clk)
+    case (CommitW svr t v cts clk lst m)
     then show ?case using Svr_Clk_le_Lst_def[of s] Finite_Pend_Inv_def[of s] Pend_Wt_LB_def[of s]
       apply (auto simp add: tps_trans_defs split: if_split_asm)
+      apply (meson le_SucI max.coboundedI1)
       by (metis Min_in empty_iff finite_pending_wtxns_removing member_remove pending_wtxns_removing)
   qed (auto simp add: tps_trans_defs)
 
 
 definition Rlst_le_Lst where
-  "Rlst_le_Lst s k \<longleftrightarrow> (\<forall>t_wr cts ts lst v rs rlst rts t.
-    svr_state (svrs s k) t_wr = Commit cts ts lst v rs \<and> rs t = Some (rts, rlst)
+  "Rlst_le_Lst s k \<longleftrightarrow> (\<forall>t_wr cts ts lst v rs rclk rlst t.
+    svr_state (svrs s k) t_wr = Commit cts ts lst v rs \<and> rs t = Some (rclk, rlst)
       \<longrightarrow> rlst \<le> svr_lst (svrs s k))"
                                                            
 lemmas Rlst_le_LstI = Rlst_le_Lst_def[THEN iffD2, rule_format]
@@ -563,20 +560,19 @@ next
   case (reach_trans s e s')
   then show ?case
   proof (induction e)
-    case (RegR x1 x2 x3 x4 x5)
+    case (RegR x1 x2 x3 x4 x5 x6 x7)
     then show ?case
       apply (auto simp add: Rlst_le_Lst_def tps_trans_defs add_to_readerset_def split: ver_state.split)
       by blast+
   next
-    case (PrepW x1 x2 x3 x4)
+    case (PrepW x1 x2 x3 x4 x5)
     then show ?case apply (auto simp add: Rlst_le_Lst_def tps_trans_defs)
       by blast
   next
-    case (CommitW x1 x2 x3 x4 x5)
-    then show ?case using svr_lst_monotonic[of s "CommitW x1 x2 x3 x4 x5" s' x1]
+    case (CommitW x1 x2 x3 x4 x5 x6 x7)
+    then show ?case using svr_lst_monotonic[of s "CommitW x1 x2 x3 x4 x5 x6 x7" s' x1]
       apply (auto simp add: Rlst_le_Lst_def tps_trans_defs)
-      using dual_order.trans apply blast
-      by (smt (z3) dual_order.trans empty_iff)
+      using dual_order.trans by blast
   qed (auto simp add: Rlst_le_Lst_def tps_trans_defs)
 qed
 
@@ -595,20 +591,18 @@ next
   case (reach_trans s e s')
   then show ?case
   proof (induction e)
-    case (RegR x1 x2 x3 x4 x5)
+    case (RegR x1 x2 x3 x4 x5 x6 x7)
     then show ?case apply (auto simp add: Get_lst_le_Lst_def tps_trans_defs)
       by (meson add_to_readerset_commit)
   next
-    case (PrepW x1 x2 x3 x4)
+    case (PrepW x1 x2 x3 x4 x5)
     then show ?case apply (auto simp add: Get_lst_le_Lst_def tps_trans_defs)
       by blast
   next
-    case (CommitW x1 x2 x3 x4 x5)
-    then show ?case using svr_lst_monotonic[of s "CommitW x1 x2 x3 x4 x5" s' x1]
+    case (CommitW x1 x2 x3 x4 x5 x6 x7)
+    then show ?case using svr_lst_monotonic[of s "CommitW x1 x2 x3 x4 x5 x6 x7" s' x1]
       apply (auto simp add: Get_lst_le_Lst_def tps_trans_defs)
-      using dual_order.trans apply blast
-      apply (smt (z3) empty_iff)
-      by (smt (z3) empty_iff sup.absorb_iff2 sup.bounded_iff)
+      using dual_order.trans by blast
   qed (auto simp add: Get_lst_le_Lst_def tps_trans_defs)
 qed
 
@@ -628,21 +622,20 @@ next
   case (reach_trans s e s')
   then show ?case
   proof (induction e)
-    case (Read x1 x2 x3 x4 x5 x6 x7 x8)
-    then show ?case apply (auto simp add: Lst_map_le_Lst_def tps_trans_defs)
+    case (Read x1 x2 x3 x4 x5 x6 x7)
+    then show ?case apply (cases x7, auto simp add: Lst_map_le_Lst_def tps_trans_defs)
       by (smt (verit) Rlst_le_Lst_def reach_rlst_le_lst)
   next
-    case (WDone x1 x2 x3 x4)
+    case (WDone x1 x2 x3 x4 x5)
     then obtain cts ts lst v rs where
       "k \<in> dom x2 \<Longrightarrow> svr_state (svrs s k) (get_wtxn s x1) = Commit cts ts lst v rs"
       by (auto simp add: tps_trans_defs, blast)
     then show ?case using WDone apply (auto simp add: Lst_map_le_Lst_def tps_trans_defs domI)
       by (smt (verit) Get_lst_le_Lst_def reach_get_lst_le_lst)
   next
-  case (CommitW x1 x2 x3 x4 x5)
-    then show ?case using svr_lst_monotonic[of s "CommitW x1 x2 x3 x4 x5" s' x1]
-      apply (auto simp add: Lst_map_le_Lst_def tps_trans_defs)
-      by (smt (z3) all_not_in_conv le_trans)
+  case (CommitW x1 x2 x3 x4 x5 x6 x7)
+    then show ?case using svr_lst_monotonic[of s "CommitW x1 x2 x3 x4 x5 x6 x7" s' x1]
+      by (auto simp add: Lst_map_le_Lst_def tps_trans_defs)
   qed (auto simp add: Lst_map_le_Lst_def tps_trans_defs)
 qed
 
@@ -663,15 +656,15 @@ next
   case (reach_trans s e s')
   then show ?case
   proof (induction e)
-    case (RegR x1 x2 x3 x4 x5)
+    case (RegR x1 x2 x3 x4 x5 x6 x7)
     then show ?case apply (auto simp add: Snapshot_R_def tps_trans_defs add_to_readerset_def
           split: ver_state.split) (* inv: x2 has not read any other versions of key x1 before *) sorry
   next
-    case (PrepW x1 x2 x3 x4)
+    case (PrepW x1 x2 x3 x4 x5)
     then show ?case apply (auto simp add: Snapshot_R_def tps_trans_defs)
       by (meson disjoint_iff_not_equal domI)
   next
-    case (CommitW x1 x2 x3 x4 x5)
+    case (CommitW x1 x2 x3 x4 x5 x6 x7)
     then show ?case apply (auto simp add: Snapshot_R_def tps_trans_defs)
       by (meson disjoint_iff_not_equal domI)
   qed (auto simp add: Snapshot_R_def tps_trans_defs)
@@ -693,8 +686,8 @@ next
   case (reach_trans s e s')
   then show ?case
   proof (induction e)
-    case (Read x1 x2 x3 x4 x5 x6 x7 x8)
-    then show ?case apply (auto simp add: Rlst_ge_Lst_map_def tps_trans_defs)
+    case (Read x1 x2 x3 x4 x5 x6 x7)
+    then show ?case apply (cases x7, auto simp add: Rlst_ge_Lst_map_def tps_trans_defs)
       using Snapshot_R_def[of s x2]
       by (metis Int_iff domI empty_iff option.inject order_class.order_eq_iff prod.inject
           reach_snapshot_r ver_state.inject(2))
@@ -703,20 +696,20 @@ next
     then show ?case apply (auto simp add: Rlst_ge_Lst_map_def tps_trans_defs)
       using Snapshot_R_def[of s] sorry
   next
-    case (WDone x1 x2 x3 x4)
+    case (WDone x1 x2 x3 x4 x5)
     then show ?case apply (auto simp add: Rlst_ge_Lst_map_def tps_trans_defs) sorry
   next
-    case (RegR x1 x2 x3 x4 x5)
+    case (RegR x1 x2 x3 x4 x5 x6 x7)
     then show ?case
       apply (auto simp add: Rlst_ge_Lst_map_def tps_trans_defs add_to_readerset_def
           split: ver_state.split)
       using reach_lst_map_le_svr_lst by blast+
   next
-    case (PrepW x1 x2 x3 x4)
+    case (PrepW x1 x2 x3 x4 x5)
     then show ?case apply (auto simp add: Rlst_ge_Lst_map_def tps_trans_defs)
       by blast
   next
-    case (CommitW x1 x2 x3 x4 x5)
+    case (CommitW x1 x2 x3 x4 x5 x6 x7)
     then show ?case apply (auto simp add: Rlst_ge_Lst_map_def tps_trans_defs)
       by blast
   qed (auto simp add: Rlst_ge_Lst_map_def tps_trans_defs)
@@ -736,23 +729,23 @@ proof(induction s rule: reach.induct)
 next
   case (reach_trans s e s')
   then show ?case
-  proof (induction e)next
-    case (Read x1 x2 x3 x4 x5 x6 x7 x8)
+  proof (induction e)
+    case (Read x1 x2 x3 x4 x5 x6 x7)
     then show ?case apply (auto simp add: Get_lst_ge_Lst_map_def tps_trans_defs) sorry
   next
     case (RDone x1 x2 x3 x4 x5)
     then show ?case apply (auto simp add: Get_lst_ge_Lst_map_def tps_trans_defs) sorry
   next
-    case (WDone x1 x2 x3 x4)
+    case (WDone x1 x2 x3 x4 x5)
     then show ?case apply (auto simp add: Get_lst_ge_Lst_map_def tps_trans_defs) sorry
   next
-    case (RegR x1 x2 x3 x4 x5)
+    case (RegR x1 x2 x3 x4 x5 x6 x7)
     then show ?case apply (auto simp add: Get_lst_ge_Lst_map_def tps_trans_defs)
       by (meson add_to_readerset_commit)
   next
-    case (CommitW x1 x2 x3 x4 x5)
+    case (CommitW x1 x2 x3 x4 x5 x6 x7)
     then show ?case apply (auto simp add: Get_lst_ge_Lst_map_def tps_trans_defs)
-      using reach_lst_map_le_svr_lst by blast
+      using reach_lst_map_le_svr_lst (*by blast*) sorry
   qed (auto simp add: Get_lst_ge_Lst_map_def tps_trans_defs)
 qed
 
@@ -762,11 +755,11 @@ lemma lst_map_monotonic:
   shows "lst_map (cls s cl) k \<le> lst_map (cls s' cl) k"
   using assms
 proof (induction e)
-  case (Read x1 x2 x3 x4 x5 x6 x7 x8)
-  then show ?case apply (auto simp add: tps_trans_defs)
+  case (Read x1 x2 x3 x4 x5 x6 x7)
+  then show ?case apply (cases x7, auto simp add: tps_trans_defs)
     using Rlst_ge_Lst_map_def[of s] reach_rlst_ge_lst_map by blast
 next
-  case (WDone x1 x2 x3 x4)
+  case (WDone x1 x2 x3 x4 x5)
   then obtain cts ts lst v rs where
     "k \<in> dom x2 \<Longrightarrow> svr_state (svrs s k) (get_wtxn s x1) = Commit cts ts lst v rs"
     by (auto simp add: tps_trans_defs, blast)
@@ -845,11 +838,11 @@ next
   case (reach_trans s e s')
   then show ?case
   proof (induction e)
-    case (Read x1 x2 x3 x4 x5 x6 x7 x8)
+    case (Read x1 x2 x3 x4 x5 x6 x7)
     then show ?case apply (simp add: Finite_Lst_map_Ran_def tps_trans_defs)
       by (meson image_mono rev_finite_subset subset_UNIV)
   next
-    case (WDone x1 x2 x3 x4)
+    case (WDone x1 x2 x3 x4 x5)
     then show ?case apply (auto simp add: Finite_Lst_map_Ran_def tps_trans_defs)
        apply (meson image_mono rev_finite_subset subset_UNIV)
         using Finite_Dom_Kv_map_def[of s x1] by (simp add: image_def dom_def)
@@ -879,13 +872,13 @@ next
   case (reach_trans s e s')
   then show ?case
   proof (induction e)
-    case (Read x1 x2 x3 x4 x5 x6 x7 x8)
-    then show ?case using lst_map_min_monotonic[of s "Read x1 x2 x3 x4 x5 x6 x7 x8" s' x1]
+    case (Read x1 x2 x3 x4 x5 x6 x7)
+    then show ?case using lst_map_min_monotonic[of s "Read x1 x2 x3 x4 x5 x6 x7" s' x1]
       apply (simp add: Gst_le_Min_Lst_map_def tps_trans_defs)
       by (smt (z3) Read.prems(1) le_trans reach.reach_trans reach_finite_lst_map_ran)
   next
-    case (WDone x1 x2 x3 x4)
-    then show ?case using lst_map_min_monotonic[of s "WDone x1 x2 x3 x4" s' x1]
+    case (WDone x1 x2 x3 x4 x5)
+    then show ?case using lst_map_min_monotonic[of s "WDone x1 x2 x3 x4 x5" s' x1]
       apply (simp add: Gst_le_Min_Lst_map_def tps_trans_defs)
       by (smt (z3) WDone.prems(1) le_trans reach.reach_trans reach_finite_lst_map_ran)
   qed (auto simp add: Gst_le_Min_Lst_map_def tps_trans_defs)
@@ -917,12 +910,12 @@ next
     then show ?case apply (simp add: Gst_le_Lst_map_def tps_trans_defs)
       by (meson Finite_Lst_map_Ran_def Min_le rangeI reach_finite_lst_map_ran)
   next
-    case (Read x1 x2 x3 x4 x5 x6 x7 x8)
-    then show ?case apply (auto simp add: Gst_le_Lst_map_def tps_trans_defs)
+    case (Read x1 x2 x3 x4 x5 x6 x7)
+    then show ?case apply (cases x7, auto simp add: Gst_le_Lst_map_def tps_trans_defs)
       by (smt (z3) Rlst_ge_Lst_map_def cl_conf.cases_scheme cl_conf.select_convs(2) le_trans
           reach_rlst_ge_lst_map reach_trans.hyps(2) txid0.inject)
   next
-    case (WDone x1 x2 x3 x4)
+    case (WDone x1 x2 x3 x4 x5)
     then obtain cts ts lst v rs where
       "k \<in> dom x2 \<Longrightarrow> svr_state (svrs s k) (get_wtxn s x1) = Commit cts ts lst v rs"
       by (auto simp add: tps_trans_defs, blast)
@@ -957,15 +950,19 @@ next
   case (reach_trans s e s')
   then show ?case
   proof (induction e)
-  case (RegR x1 x2 x3 x4 x5)
+  case (RegR x1 x2 x3 x4 x5 x6 x7)
   then show ?case apply (auto simp add: Lst_Lt_Pts_def tps_trans_defs)
     by (meson add_to_readerset_prep_inv)
   next
-    case (CommitW x1 x2 x3 x4 x5)
+    case (PrepW x1 x2 x3 x4 x5)
     then show ?case apply (auto simp add: Lst_Lt_Pts_def tps_trans_defs)
-      apply (metis emptyE other_prep_t_inv)
-      by (metis Finite_Pend_Inv_def Min.coboundedI finite_pending_wtxns_removing other_prep_t_inv
-          reach_finitepending)
+      by (meson Svr_Clk_le_Lst_def le_SucI le_trans max.cobounded1 reach_svr_clock_svr_lst_inv)
+  next
+    case (CommitW x1 x2 x3 x4 x5 x6 x7)
+    then show ?case apply (auto simp add: Lst_Lt_Pts_def tps_trans_defs)
+      using Pend_Wt_LB_def[of s' x1] pending_wtxns_ts_def apply auto
+      apply (smt (z3) other_prep_t_inv)
+      by (smt (z3) CommitW.prems(1) reach.reach_trans reach_pend_wt_lb)
   qed(auto simp add: Lst_Lt_Pts_def tps_trans_defs)
 qed
 
@@ -984,7 +981,7 @@ next
   case (reach_trans s e s')
   then show ?case
   proof (induction e)
-    case (RegR x1 x2 x3 x4 x5)
+    case (RegR x1 x2 x3 x4 x5 x6 x7)
     then show ?case
       by (auto simp add: Finite_Wtxns_Dom_def tps_trans_defs add_to_readerset_def
                split: ver_state.split)
@@ -1005,7 +1002,7 @@ next
   case (reach_trans s e s')
   then show ?case
   proof (induction e)
-    case (RegR x1 x2 x3 x4 x5)
+    case (RegR x1 x2 x3 x4 x5 x6 x7)
     then show ?case
       by (auto simp add: Finite_Wtxns_rsran_def tps_trans_defs add_to_readerset_def
                split: ver_state.split)
@@ -1031,17 +1028,17 @@ next
   case (reach_trans s e s')
   then show ?case
   proof (induction e)
-    case (RegR x1 x2 x3 x4 x5)
+    case (RegR x1 x2 x3 x4 x5 x6 x7)
     then show ?case
       apply (auto simp add: Kvs_Not_Emp_def tps_trans_defs)
       by (metis add_to_readerset_wtxns_dom wtxns_domIff)
   next
-    case (PrepW x1 x2 x3 x4)
+    case (PrepW x1 x2 x3 x4 x5)
     then show ?case
       apply (auto simp add: Kvs_Not_Emp_def tps_trans_defs)
       by (metis fun_upd_same ver_state.distinct(1))
   next
-    case (CommitW x1 x2 x3 x4 x5)
+    case (CommitW x1 x2 x3 x4 x5 x6 x7)
     then show ?case
       apply (auto simp add: Kvs_Not_Emp_def tps_trans_defs)
       by (metis fun_upd_same ver_state.distinct(3))
@@ -1064,7 +1061,7 @@ next
   case (reach_trans s e s')
   then show ?case
   proof (induction e)
-    case (WCommit x1 x2 x3 x4 x5 x6)
+    case (WCommit x1 x2 x3 x4 x5 x6 x7)
     then show ?case apply (auto simp add: T0_in_CO_def tps_trans_all_defs)
       by (smt (verit) in_set_remove1 remove1_insort_key txid.distinct(1))
   qed (auto simp add: T0_in_CO_def tps_trans_defs)
@@ -1096,7 +1093,7 @@ next
   case (reach_trans s e s')
   then show ?case
   proof (induction e)
-    case (RegR x1 x2 x3 x4 x5)
+    case (RegR x1 x2 x3 x4 x5 x6 x7)
     then show ?case apply (simp add: Init_Ver_Inv_def tps_trans_defs)
       by (meson add_to_readerset_commit')
   qed (auto simp add: Init_Ver_Inv_def tps_trans_defs)
@@ -1137,7 +1134,7 @@ next
   case (reach_trans s e s')
   then show ?case 
   proof (induction e)
-    case (RegR x71 x72 x73 x74)
+    case (RegR x71 x72 x73 x74 x75 x76 x77)
     then show ?case
       apply (auto simp add: tps_trans_defs FTid_Wtxn_Inv_def)
       by (metis add_to_readerset_no_ver_inv)
@@ -1161,15 +1158,15 @@ next
   case (reach_trans s e s')
   then show ?case 
   proof (induction e)
-    case (RegR x1 x2 x3 x4 x5)
+    case (RegR x1 x2 x3 x4 x5 x6 x7)
     then show ?case apply (simp add: Cl_Rtxn_Inv_def tps_trans_defs)
       by (metis add_to_readerset_no_ver_inv)
   next
-    case (PrepW x1 x2 x3 x4)
+    case (PrepW x1 x2 x3 x4 x5)
     then show ?case apply (simp add: Cl_Rtxn_Inv_def tps_trans_defs)
       by (metis get_cl_w.simps(2) txn_state.distinct(3) txn_state.distinct(7) txid0.collapse)
   next
-    case (CommitW x1 x2 x3 x4 x5)
+    case (CommitW x1 x2 x3 x4 x5 x6 x7)
     then show ?case apply (simp add: Cl_Rtxn_Inv_def tps_trans_defs)
       by force
   qed (auto simp add: Cl_Rtxn_Inv_def tps_trans_defs)
@@ -1192,15 +1189,15 @@ next
   case (reach_trans s e s')
   then show ?case 
   proof (induction e)
-    case (RegR x1 x2 x3 x4 x5)
+    case (RegR x1 x2 x3 x4 x5 x6 x7)
     then show ?case apply (simp add: Cl_Wtxn_Idle_Svr_def tps_trans_defs)
       by (metis add_to_readerset_no_ver_inv)
   next
-    case (PrepW x1 x2 x3 x4)
+    case (PrepW x1 x2 x3 x4 x5)
     then show ?case apply (simp add: Cl_Wtxn_Idle_Svr_def tps_trans_defs)
       by (smt (z3) domIff get_cl_w.simps(2) txn_state.distinct(11) txn_state.inject(2) txid0.collapse)
   next
-    case (CommitW x1 x2 x3 x4 x5)
+    case (CommitW x1 x2 x3 x4 x5 x6 x7)
     then show ?case apply (simp add: Cl_Wtxn_Idle_Svr_def tps_trans_defs)
       by force
   qed (auto simp add: Cl_Wtxn_Idle_Svr_def tps_trans_defs, blast?)
@@ -1226,15 +1223,15 @@ next
     case (WInvoke x1 x2 x3 x4)
     then show ?case by (simp add: Cl_Prep_Inv_def tps_trans_defs, blast)
   next
-    case (RegR x1 x2 x3 x4 x5)
+    case (RegR x1 x2 x3 x4 x5 x6 x7)
     then show ?case apply (simp add: Cl_Prep_Inv_def tps_trans_defs)
       by (smt (verit) add_to_readerset_wtxns_dom add_to_readerset_prep_inv wtxns_domIff)
   next
-    case (PrepW x1 x2 x3 x4)
+    case (PrepW x1 x2 x3 x4 x5)
     then show ?case apply (simp add: Cl_Prep_Inv_def tps_trans_defs)
       by (metis domI get_cl_w.simps(2) txn_state.inject(2) txid0.collapse)
   next
-    case (CommitW x1 x2 x3 x4 x5)
+    case (CommitW x1 x2 x3 x4 x5 x6 x7)
     then show ?case apply (simp add: Cl_Prep_Inv_def tps_trans_defs)
       using get_cl_w.simps(2) txn_state.distinct(11) txn_state.simps(19) by force
   qed (auto simp add: Cl_Prep_Inv_def tps_trans_defs)
@@ -1258,20 +1255,20 @@ next
   case (reach_trans s e s')
   then show ?case 
   proof (induction e)
-    case (WCommit x1 x2 x3 x4 x5 x6)
+    case (WCommit x1 x2 x3 x4 x5 x6 x7)
     then show ?case apply (simp add: Cl_Commit_Inv_def tps_trans_defs)
       by (metis (no_types, lifting) Cl_Prep_Inv_def domI domIff option.inject reach_cl_prep_inv)
   next
-    case (RegR x1 x2 x3 x4 x5)
+    case (RegR x1 x2 x3 x4 x5 x6 x7)
     then show ?case apply (simp add: Cl_Commit_Inv_def tps_trans_defs)
       by (smt add_to_readerset_commit add_to_readerset_no_ver_inv add_to_readerset_prep_inv
           ver_state.exhaust ver_state.inject(2))
   next
-    case (PrepW x1 x2 x3 x4)
+    case (PrepW x1 x2 x3 x4 x5)
     then show ?case apply (simp add: Cl_Commit_Inv_def tps_trans_defs)
       by (smt (verit) fun_upd_other get_cl_w.simps(2) txn_state.distinct(11) txid0.collapse)
   next
-    case (CommitW x1 x2 x3 x4 x5)
+    case (CommitW x1 x2 x3 x4 x5 x6 x7)
     then show ?case apply (simp add: Cl_Commit_Inv_def tps_trans_defs)
       by (metis domD get_cl_w.simps(2) txn_state.inject(3) ver_state.distinct(5) ver_state.inject(1) txid0.collapse)
   qed (auto simp add: Cl_Commit_Inv_def tps_trans_defs)
@@ -1298,19 +1295,20 @@ next
       by (metis Cl_Rtxn_Inv_def get_cl_w.elims get_sn_w.simps(2) insert_iff is_prepared.simps(2)
           reach_cl_rtxn_inv)
   next
-    case (WDone x1 x2 x3 x4)
+    case (WDone x1 x2 x3 x4 x5)
     then show ?case apply (auto simp add: Prep_is_Curr_wt_def tps_trans_defs)
     apply (cases "x2 k")
        apply (smt (z3) Cl_Wtxn_Idle_Svr_def get_cl_w.simps(2) get_sn_w.cases get_sn_w.simps(2)
           insert_commute insert_compr insert_iff is_prepared.elims(1) reach_cl_wtxn_idle_svr
           ver_state.distinct(1))
-      by (metis domI get_cl_w.elims get_sn_w.simps(2) is_prepared.simps(3))
+      by (smt domI get_cl_w.simps(2) get_sn_w.cases get_sn_w.simps(2) is_prepared.simps(3)
+          mem_Collect_eq option.discI)
   next
-    case (RegR x1 x2 x3 x4 x5)
+    case (RegR x1 x2 x3 x4 x5 x6 x7)
     then show ?case apply (simp add: Prep_is_Curr_wt_def tps_trans_defs)
       by (smt (verit, ccfv_SIG) add_to_readerset_prep_inv is_prepared.elims(2))
   next
-    case (PrepW x1 x2 x3 x4)
+    case (PrepW x1 x2 x3 x4 x5)
     then show ?case apply (simp add: Prep_is_Curr_wt_def tps_trans_defs)
       by (metis get_cl_w.simps(2) get_sn_w.simps(2) txid0.collapse)
   qed (auto simp add: Prep_is_Curr_wt_def tps_trans_defs)
@@ -1337,7 +1335,7 @@ next
     then show ?case apply (simp add: Svr_Prep_Inv_def tps_trans_defs)
       by (metis txn_state.distinct(3) txn_state.distinct(5))
   next
-    case (Read x1 x2 x3 x4 x5 x6 x7 x8)
+    case (Read x1 x2 x3 x4 x5 x6 x7)
     then show ?case apply (simp add: Svr_Prep_Inv_def tps_trans_defs)
       by (metis txn_state.distinct(7) txn_state.distinct(9))
   next
@@ -1349,20 +1347,20 @@ next
     then show ?case apply (simp add: Svr_Prep_Inv_def tps_trans_defs)
       by (metis txn_state.distinct(3) txn_state.distinct(5))
   next
-    case (WCommit x1 x2 x3 x4 x5 x6)
+    case (WCommit x1 x2 x3 x4 x5 x6 x7)
     then show ?case apply (simp add: Svr_Prep_Inv_def tps_trans_defs)
       by (metis (lifting) txn_state.distinct(11) txn_state.inject(2))
   next
-    case (WDone x1 x2 x3 x4)
+    case (WDone x1 x2 x3 x4 x5)
     then show ?case apply (simp add: Svr_Prep_Inv_def tps_trans_defs)
       by (metis (no_types, lifting) Prep_is_Curr_wt_def get_cl_w.elims get_sn_w.simps(2)
           is_prepared.simps(1) reach_prep_is_curr_wt txn_state.distinct(11) txn_state.inject(3)
           ver_state.distinct(5))
   next
-    case (RegR x1 x2 x3 x4 x5)
+    case (RegR x1 x2 x3 x4 x5 x6 x7)
     then show ?case by (simp add: Svr_Prep_Inv_def tps_trans_defs add_to_readerset_prep_inv)
   next
-    case (PrepW x1 x2 x3 x4)
+    case (PrepW x1 x2 x3 x4 x5)
     then show ?case apply (simp add: Svr_Prep_Inv_def tps_trans_defs)
       by (metis domI get_cl_w.simps(2) txid0.collapse)
   qed (auto simp add: Svr_Prep_Inv_def tps_trans_defs)
@@ -1389,7 +1387,7 @@ next
     then show ?case apply (simp add: Svr_Commit_Inv_def tps_trans_defs)
       by (metis txn_state.distinct(5))
   next
-    case (Read x1 x2 x3 x4 x5 x6 x7 x8)
+    case (Read x1 x2 x3 x4 x5 x6 x7)
     then show ?case apply (simp add: Svr_Commit_Inv_def tps_trans_defs)
       by (metis txn_state.distinct(9))
   next
@@ -1402,20 +1400,20 @@ next
     then show ?case apply (simp add: Svr_Commit_Inv_def tps_trans_defs)
       by (metis txn_state.distinct(5))
   next
-    case (WCommit x1 x2 x3 x4 x5 x6)
+    case (WCommit x1 x2 x3 x4 x5 x6 x7)
     then show ?case apply (simp add: Svr_Commit_Inv_def tps_trans_defs)
       by (metis (lifting) txn_state.distinct(11))
   next
-    case (WDone x1 x2 x3 x4)
+    case (WDone x1 x2 x3 x4 x5)
     then show ?case apply (auto simp add: Svr_Commit_Inv_def tps_trans_defs)
       by (metis (lifting) FTid_Wtxn_Inv_def get_cl_w.elims get_sn_w.simps(2)
           lessI reach_ftid_wtxn_inv ver_state.distinct(3))
   next
-    case (RegR x1 x2 x3 x4 x5)
+    case (RegR x1 x2 x3 x4 x5 x6 x7)
     then show ?case apply (auto simp add: Svr_Commit_Inv_def tps_trans_defs)
     by (metis add_to_readerset_commit)
   next
-    case (CommitW x1 x2 x3 x4 x5)
+    case (CommitW x1 x2 x3 x4 x5 x6 x7)
     then show ?case apply (auto simp add: Svr_Commit_Inv_def tps_trans_defs)
       by (metis domI get_cl_w.simps(2) txid0.collapse)
   qed (auto simp add: Svr_Commit_Inv_def tps_trans_defs)
@@ -1458,7 +1456,7 @@ next
         by (metis (no_types, lifting) domIff less_antisym)
       done
   next
-    case (RegR x71 x72 x73 x74)
+    case (RegR x71 x72 x73 x74 x75 x76 x77)
     then show ?case
       apply (auto simp add: tps_trans_defs PTid_Inv_def)
       apply (metis add_to_readerset_no_ver_inv)
@@ -1495,11 +1493,11 @@ next
     then show ?case apply (simp add: Rtxn_Wtxn_No_Ver_def tps_trans_defs)
       using Cl_Rtxn_Inv_def by blast
   next
-    case (RegR x1 x2 x3 x4 x5)
+    case (RegR x1 x2 x3 x4 x5 x6 x7)
     then show ?case apply (simp add: Rtxn_Wtxn_No_Ver_def tps_trans_defs)
       by (meson add_to_readerset_no_ver_inv)
   next
-    case (PrepW x1 x2 x3 x4)
+    case (PrepW x1 x2 x3 x4 x5)
     then show ?case apply (auto simp add: Rtxn_Wtxn_No_Ver_def tps_trans_defs)
       by (metis CFTid_Rtxn_Inv_def get_sn_w.simps(2) le_refl reach_cftid_rtxn_inv)
   qed (auto simp add: Rtxn_Wtxn_No_Ver_def tps_trans_defs)
@@ -1521,16 +1519,16 @@ next
   case (reach_trans s e s')
   then show ?case using Cl_Rtxn_Inv_def[of s]
   proof (induction e)
-    case (RegR x1 x2 x3 x4 x5)
+    case (RegR x1 x2 x3 x4 x5 x6 x7)
     then show ?case apply (simp add: Wtxn_Rtxn_None_def tps_trans_defs)
       by (meson add_to_readerset_commit_subset add_to_readerset_prep_inv)
   next
-    case (PrepW x1 x2 x3 x4)
+    case (PrepW x1 x2 x3 x4 x5)
     then show ?case apply (simp add: Wtxn_Rtxn_None_def tps_trans_defs)
       by (metis CFTid_Rtxn_Inv_def get_cl_w.simps(2) get_sn_w.simps(2) le_refl
           reach_cftid_rtxn_inv txid0.collapse)
   next
-    case (CommitW x1 x2 x3 x4 x5)
+    case (CommitW x1 x2 x3 x4 x5 x6 x7)
     then show ?case apply (simp add: Wtxn_Rtxn_None_def tps_trans_defs)
       by (meson is_prepared.elims(2))
   qed (auto simp add: Wtxn_Rtxn_None_def tps_trans_defs)
@@ -1625,7 +1623,7 @@ next
   case (reach_trans s e s')
   then show ?case
   proof (induction e)
-    case (WCommit x1 x2 x3 x4 x5 x6)
+    case (WCommit x1 x2 x3 x4 x5 x6 x7)
     then show ?case apply (auto simp add: Wtxn_State_Cts_def tps_trans_defs domI)
       apply (metis (no_types, lifting) Cl_Prep_Inv_def reach_cl_prep_inv ver_state.distinct(3)
           ver_state.distinct(5))
@@ -1634,15 +1632,15 @@ next
       by (metis Prep_is_Curr_wt_def get_cl_w.simps(2) get_sn_w.cases get_sn_w.simps(2)
           is_prepared.simps(1) reach_prep_is_curr_wt).
   next
-    case (RegR x1 x2 x3 x4 x5)
+    case (RegR x1 x2 x3 x4 x5 x6 x7)
     then show ?case apply (simp add: Wtxn_State_Cts_def tps_trans_defs domI)
       by (meson add_to_readerset_commit add_to_readerset_prep_inv)
   next
-    case (PrepW x1 x2 x3 x4)
+    case (PrepW x1 x2 x3 x4 x5)
     then show ?case apply (simp add: Wtxn_State_Cts_def tps_trans_defs domI)
       by (metis get_cl_w.simps(2) txid0.exhaust_sel txn_state.distinct(11))
   next
-    case (CommitW x1 x2 x3 x4 x5)
+    case (CommitW x1 x2 x3 x4 x5 x6 x7)
     then show ?case apply (simp add: Wtxn_State_Cts_def tps_trans_defs domI)
       by (metis get_cl_w.simps(2) txid0.collapse)
   qed (auto simp add: Wtxn_State_Cts_def tps_trans_defs domI)
@@ -1667,20 +1665,20 @@ next
     then show ?case apply (simp add: FTid_notin_rs_def tps_trans_defs)
       by (meson Suc_lessD)
   next
-    case (WDone x1 x2 x3 x4)
+    case (WDone x1 x2 x3 x4 x5)
     then show ?case apply (simp add: FTid_notin_rs_def tps_trans_defs)
       by (meson Suc_lessD)
   next
-    case (RegR x1 x2 x3 x4 x5)
+    case (RegR x1 x2 x3 x4 x5 x6 x7)
     then show ?case apply (simp add: FTid_notin_rs_def tps_trans_defs add_to_readerset_def
           split: ver_state.split)
       by (smt (verit) less_irrefl_nat txid0.sel(1) txid0.sel(2))
   next
-    case (PrepW x1 x2 x3 x4)
+    case (PrepW x1 x2 x3 x4 x5)
     then show ?case apply (simp add: FTid_notin_rs_def tps_trans_defs)
       by (metis)
   next
-    case (CommitW x1 x2 x3 x4 x5)
+    case (CommitW x1 x2 x3 x4 x5 x6 x7)
     then show ?case apply (simp add: FTid_notin_rs_def tps_trans_defs)
       by (smt empty_iff fun_upd_other fun_upd_same txn_state.simps(19) ver_state.inject(2)
           ver_state.simps(10))
@@ -1710,15 +1708,15 @@ next
     then show ?case apply (simp add: FTid_not_wr_def tps_trans_defs)
       by (metis Suc_lessD)
   next
-    case (RegR x1 x2 x3 x4 x5)
+    case (RegR x1 x2 x3 x4 x5 x6 x7)
     then show ?case apply (simp add: FTid_not_wr_def tps_trans_defs)
       by (simp add: add_to_readerset_wtxns_dom)
   next
-    case (PrepW x81 x82 x83)
+    case (PrepW x81 x82 x83 x84 x85)
     then show ?case apply (simp add: FTid_not_wr_def tps_trans_defs)
       by (metis get_cl_w.simps(2) get_sn_w.simps(2) nat_neq_iff txid0.collapse)
   next
-    case (CommitW x91 x92)
+    case (CommitW x91 x92 x93 x94 x95 x96 x97)
     then show ?case apply (simp add: FTid_not_wr_def tps_trans_defs)
       by (metis get_cl_w.simps(2) get_sn_w.simps(2) order_less_irrefl txid0.collapse)
   qed (auto simp add: FTid_not_wr_def tps_trans_defs)
@@ -1744,11 +1742,11 @@ next
     then show ?case apply (auto simp add: Fresh_wr_notin_rs_def tps_trans_defs)
       using FTid_notin_rs_def lessI by blast
   next
-    case (WDone x1 x2 x3 x4)
+    case (WDone x1 x2 x3 x4 x5)
     then show ?case apply (auto simp add: Fresh_wr_notin_rs_def tps_trans_defs)
       using FTid_notin_rs_def by blast
   next
-    case (RegR x1 x2 x3 x4 x5)
+    case (RegR x1 x2 x3 x4 x5 x6 x7)
     then show ?case by (auto simp add: Fresh_wr_notin_rs_def tps_trans_defs add_to_readerset_def
           split: ver_state.split)
   qed (auto simp add: Fresh_wr_notin_rs_def tps_trans_defs split: txn_state.split)
@@ -1770,11 +1768,11 @@ next
   case (reach_trans s e s')
   then show ?case 
   proof (induction e)
-    case (RegR x1 x2 x3 x4 x5)
+    case (RegR x1 x2 x3 x4 x5 x6 x7)
     then show ?case apply (simp add: tps_trans_defs Fresh_wr_notin_Wts_dom_def)
       by (metis add_to_readerset_wtxns_dom)
   next
-    case (PrepW x1 x2 x3 x4)
+    case (PrepW x1 x2 x3 x4 x5)
     then show ?case apply (simp add: tps_trans_defs Fresh_wr_notin_Wts_dom_def)
       by (metis get_cl_w.simps(2) txn_state.distinct(3) txn_state.distinct(7) txid0.collapse)
   qed (auto simp add: tps_trans_defs Fresh_wr_notin_Wts_dom_def)
@@ -1826,18 +1824,19 @@ next
     then show ?case apply (simp add: Gst_le_Pts_def tps_trans_defs)
       by (meson FTid_not_wr_def lessI reach_ftid_not_wr wtxns_domI1)
   next
-    case (WDone x1 x2 x3 x4)
+    case (WDone x1 x2 x3 x4 x5)
     then show ?case apply (simp add: Gst_le_Pts_def tps_trans_defs)
       by (meson FTid_not_wr_def less_Suc_eq reach_ftid_not_wr wtxns_domI1)
   next
-    case (RegR x1 x2 x3 x4 x5)
+    case (RegR x1 x2 x3 x4 x5 x6 x7)
     then show ?case apply (simp add: Gst_le_Pts_def tps_trans_defs)
       by (meson add_to_readerset_prep_inv)
   next
-    case (PrepW x1 x2 x3 x4)
+    case (PrepW x1 x2 x3 x4 x5)
     then show ?case apply (auto simp add: Gst_le_Pts_def tps_trans_defs)
-      using Gst_le_Lst_map_def[of s cl x1] Lst_map_le_Lst_def Svr_Clk_le_Lst_def
-      by (metis dual_order.trans reach_svr_clock_svr_lst_inv reach_gst_le_svr_lst reach_lst_map_le_svr_lst)
+      using Gst_le_Lst_map_def Lst_map_le_Lst_def Svr_Clk_le_Lst_def
+      by (metis le_SucI le_trans max.coboundedI1 reach_gst_le_svr_lst reach_lst_map_le_svr_lst
+          reach_svr_clock_svr_lst_inv)
   qed (auto simp add: Gst_le_Pts_def tps_trans_defs)
 qed
 
@@ -1866,15 +1865,15 @@ next
     then show ?case apply (simp add: Gst_Lt_Cts_def tps_trans_defs)
       by (metis FTid_Wtxn_Inv_def lessI reach_ftid_wtxn_inv ver_state.distinct(3))
   next
-    case (WDone x1 x2 x3 x4)
+    case (WDone x1 x2 x3 x4 x5)
     then show ?case apply (simp add: Gst_Lt_Cts_def tps_trans_defs)
       by (meson FTid_not_wr_def less_Suc_eq reach_ftid_not_wr wtxns_domI2)
   next
-    case (RegR x1 x2 x3 x4 x5)
+    case (RegR x1 x2 x3 x4 x5 x6 x7)
     then show ?case apply (simp add: Gst_Lt_Cts_def tps_trans_defs)
       by (meson add_to_readerset_commit)
   next
-    case (CommitW x1 x2 x3 x4 x5)
+    case (CommitW x1 x2 x3 x4 x5 x6 x7)
     then show ?case apply (simp add: Gst_Lt_Cts_def tps_trans_defs) sorry
   qed (auto simp add: Gst_Lt_Cts_def tps_trans_defs)
 qed
@@ -1899,41 +1898,10 @@ next
     case (RInvoke x1 x2 x3 x4)
     then show ?case apply (auto simp add: Gst_Lt_Cl_Cts_def tps_trans_defs) sorry
   next
-    case (WCommit x1 x2 x3 x4 x5 x6)
+    case (WCommit x1 x2 x3 x4 x5 x6 x7)
     then show ?case apply (auto simp add: Gst_Lt_Cl_Cts_def tps_trans_defs)
       apply (cases "cl = x1"; simp) sorry
   qed (auto simp add: Gst_Lt_Cl_Cts_def tps_trans_defs, (blast+)?)
-qed
-
-definition Cl_Cts_lt_Wtxn_Cts where
-  "Cl_Cts_lt_Wtxn_Cts s cl \<longleftrightarrow> (\<forall>cts sn kv_map. cl_state (cls s cl) = WtxnPrep kv_map \<and>
-    wtxn_cts s (Tn (Tn_cl sn cl)) = Some cts \<longrightarrow>
-    cts < max (cl_clock (cls s cl)) (Max {get_ts (svr_state (svrs s k) (get_wtxn s cl)) |k. k \<in> dom kv_map}))"
-
-lemmas Cl_Cts_lt_Wtxn_CtsI = Cl_Cts_lt_Wtxn_Cts_def[THEN iffD2, rule_format]
-lemmas Cl_Cts_lt_Wtxn_CtsE[elim] = Cl_Cts_lt_Wtxn_Cts_def[THEN iffD1, elim_format, rule_format]
-
-lemma reach_cl_cts_lt_wtxn_cts [simp, dest]: "reach tps_s s \<Longrightarrow> Cl_Cts_lt_Wtxn_Cts s cl"
-proof(induction s rule: reach.induct)
-  case (reach_init s)
-  then show ?case
-    by (auto simp add: Cl_Cts_lt_Wtxn_Cts_def tps_s_defs)
-next
-  case (reach_trans s e s')
-  then show ?case
-  proof (induction e)
-    case (WInvoke x1 x2 x3 x4)
-    then show ?case apply (auto simp add: Cl_Cts_lt_Wtxn_Cts_def tps_trans_defs) sorry
-  next
-    case (RegR x1 x2 x3 x4 x5)
-    then show ?case apply (auto simp add: Cl_Cts_lt_Wtxn_Cts_def tps_trans_defs) sorry
-  next
-    case (PrepW x1 x2 x3 x4)
-    then show ?case apply (auto simp add: Cl_Cts_lt_Wtxn_Cts_def tps_trans_defs) sorry
-  next
-    case (CommitW x1 x2 x3 x4 x5)
-    then show ?case apply (auto simp add: Cl_Cts_lt_Wtxn_Cts_def tps_trans_defs) sorry
-  qed (auto simp add: Cl_Cts_lt_Wtxn_Cts_def tps_trans_defs)
 qed
 
 subsection \<open>Commit Timestamps Order Invariants\<close>
@@ -1959,14 +1927,14 @@ next
     then show ?case apply (simp add: CO_Tid_def tps_trans_defs split: txn_state.split_asm)
       using less_SucI less_Suc_eq_le by blast+
   next
-    case (WCommit x1 x2 x3 x4 x5 x6)
+    case (WCommit x1 x2 x3 x4 x5 x6 x7)
     then show ?case apply (simp add: CO_Tid_def tps_trans_all_defs set_insort_key split: txn_state.split_asm)
       apply (metis txn_state.distinct(3))
       apply (metis txn_state.distinct(7))
       apply (meson less_or_eq_imp_le)
       by blast
   next
-    case (WDone x1 x2 x3 x4)
+    case (WDone x1 x2 x3 x4 x5)
     then show ?case apply (simp add: CO_Tid_def tps_trans_defs split: txn_state.split_asm)
       apply (meson less_SucI)+
       by (meson linorder_le_less_linear not_less_eq_eq)
@@ -1988,7 +1956,7 @@ next
   case (reach_trans s e s')
   then show ?case
   proof (induction e)
-    case (WCommit x1 x2 x3 x4 x5 x6)
+    case (WCommit x1 x2 x3 x4 x5 x6 x7)
     then show ?case apply (auto simp add: CO_Distinct_def tps_trans_all_defs distinct_insort)
       by (metis (no_types, lifting) CO_Tid_def less_irrefl_nat reach_co_tid txn_state.simps(18))
   qed (simp_all add: CO_Distinct_def tps_trans_defs)
@@ -2017,7 +1985,7 @@ next
     then show ?case apply (simp add: CO_Tn_is_Cmt_Abs_def tps_trans_defs)
       by (metis txn_state.distinct(5))
   next
-    case (Read x1 x2 x3 x4 x5 x6 x7 x8)
+    case (Read x1 x2 x3 x4 x5 x6 x7)
     then show ?case apply (simp add: CO_Tn_is_Cmt_Abs_def tps_trans_defs)
       by (metis txn_state.distinct(9))
   next
@@ -2029,23 +1997,23 @@ next
     then show ?case apply (simp add: CO_Tn_is_Cmt_Abs_def tps_trans_defs)
       by (metis txn_state.distinct(5))
   next
-    case (WCommit x1 x2 x3 x4 x5 x6)
+    case (WCommit x1 x2 x3 x4 x5 x6 x7)
     then show ?case apply (simp add: CO_Tn_is_Cmt_Abs_def tps_trans_all_defs set_insort_key)
       by (smt (verit) domIff is_prepared.elims(2) option.discI txn_state.distinct(11))
   next
-    case (WDone x1 x2 x3 x4)
+    case (WDone x1 x2 x3 x4 x5)
     then show ?case apply (simp add: CO_Tn_is_Cmt_Abs_def tps_trans_defs)
       by (metis (no_types, lifting) txn_state.inject(3))
   next
-    case (RegR x1 x2 x3 x4 x5)
+    case (RegR x1 x2 x3 x4 x5 x6 x7)
     then show ?case apply (simp add: CO_Tn_is_Cmt_Abs_def tps_trans_defs)
       by (metis add_to_readerset_commit' add_to_readerset_prep_inv)
   next
-    case (PrepW x1 x2 x3 x4)
+    case (PrepW x1 x2 x3 x4 x5)
     then show ?case apply (simp add: CO_Tn_is_Cmt_Abs_def tps_trans_defs)
       by (metis ver_state.distinct(3))
   next
-    case (CommitW x1 x2 x3 x4 x5)
+    case (CommitW x1 x2 x3 x4 x5 x6 x7)
     then show ?case apply (simp add: CO_Tn_is_Cmt_Abs_def tps_trans_defs)
       by (smt (z3) fun_upd_apply txn_state.simps(19) ver_state.simps(10))
   qed
@@ -2109,19 +2077,19 @@ next
   case (reach_trans s e s')
   then show ?case
   proof (induction e)
-    case (Read x1 x2 x3 x4 x5 x6 x7 x8)
+    case (Read x1 x2 x3 x4 x5 x6 x7)
     then show ?case apply (simp add: Committed_Abs_Tn_in_CO_def tps_trans_defs)
       by (metis txn_state.distinct(9) txn_state.simps(17))
   next
-    case (WCommit x1 x2 x3 x4 x5 x6)
+    case (WCommit x1 x2 x3 x4 x5 x6 x7)
     then show ?case apply (simp add: Committed_Abs_Tn_in_CO_def tps_trans_all_defs set_insort_key)
       by (metis (no_types, lifting) Cl_Prep_Inv_def domIff reach_cl_prep_inv ver_state.distinct(1))
   next
-    case (RegR x1 x2 x3 x4 x5)
+    case (RegR x1 x2 x3 x4 x5 x6 x7)
     then show ?case apply (simp add: Committed_Abs_Tn_in_CO_def tps_trans_defs)
       by (smt (verit) add_to_readerset_commit add_to_readerset_prep_inv)
   next
-    case (PrepW x1 x2 x3 x4)
+    case (PrepW x1 x2 x3 x4 x5)
     then show ?case apply (simp add: Committed_Abs_Tn_in_CO_def tps_trans_defs)
       by (metis get_cl_w.simps(2) txn_state.distinct(11) txid0.collapse)
   qed (auto simp add: Committed_Abs_Tn_in_CO_def tps_trans_defs)
@@ -2158,7 +2126,7 @@ next
   case (reach_trans s e s')
   then show ?case 
   proof (induction e)
-    case (WCommit x1 x2 x3 x4 x5 x6)
+    case (WCommit x1 x2 x3 x4 x5 x6 x7)
     then have indom: "k \<in> dom x2 \<Longrightarrow> cts_order s' k = cts_order s k @ [get_wtxn s x1]"
       apply (auto simp add: tps_trans_all_defs) (* CONTINUE! *) sorry
     have nindom: "k \<notin> dom x2 \<Longrightarrow> cts_order s' k = cts_order s k" using WCommit
@@ -2192,7 +2160,7 @@ next
   case (reach_trans s e s')
   then show ?case
   proof (induction e)
-    case (WCommit x1 x2 x3 x4 x5 x6)
+    case (WCommit x1 x2 x3 x4 x5 x6 x7)
     then show ?case apply (auto simp add: T0_First_in_CO_def tps_trans_all_defs)
       using T0_min_unique_ts[of s] T0_in_CO_def[of s] append_Cons empty_iff empty_set neq_Nil_conv nth_Cons_0 reach_t0_in_co sorry (* Continue here! *)
   qed (auto simp add: T0_First_in_CO_def tps_trans_all_defs)
@@ -2264,10 +2232,10 @@ next
       apply (simp add: read_done_def read_done_U_def) sorry
     then show ?case using RDone sqn_added by (auto simp add: Sqn_Inv_nc_def tps_trans_defs)
   next
-    case (WCommit x1 x2 x3 x4 x5 x6)
+    case (WCommit x1 x2 x3 x4 x5 x6 x7)
     then show ?case apply (simp add: Sqn_Inv_nc_def tps_trans_defs) sorry
   next
-    case (WDone x1 x2 x3 x4)
+    case (WDone x1 x2 x3 x4 x5)
     then show ?case apply (simp add: Sqn_Inv_nc_def tps_trans_defs)
       by (metis less_SucI nat.discI txn_state.inject(3))
   qed (auto simp add: Sqn_Inv_nc_def tps_trans_defs)
@@ -2294,7 +2262,7 @@ next
       by (metis (full_types) Sqn_Inv_nc_def gt_ex nless_le reach.reach_trans reach_sql_inv_nc
           reach_trans.hyps(1) txn_state.inject(3))+
   next
-    case (WCommit x1 x2 x3 x4 x5 x6)
+    case (WCommit x1 x2 x3 x4 x5 x6 x7)
     then show ?case apply (simp add: Sqn_Inv_c_def)
       by (metis Sqn_Inv_nc_def less_or_eq_imp_le reach.reach_trans reach_sql_inv_nc
           reach_trans.hyps(1) txn_state.inject(3))
@@ -2431,7 +2399,7 @@ next
       using Fresh_wr_notin_rs_def[of s]
       by (metis insertCI reach_fresh_wr_notin_rs)
   next
-    case (RegR x1 x2 x3 x4 x5)
+    case (RegR x1 x2 x3 x4 x5 x6 x7)
     then show ?case 
       by (auto simp add: Rtxn_IdleK_notin_rs_def tps_trans_defs add_to_readerset_def
                split: ver_state.split)
@@ -2454,21 +2422,21 @@ next
   case (reach_trans s e s')
   then show ?case 
   proof (induction e)
-    case (Read x1 x2 x3 x4 x5 x6 x7 x8)
-    then show ?case apply (auto simp add: Rtxn_RegK_Kvtm_Cmt_in_rs_def tps_trans_defs)
+    case (Read x1 x2 x3 x4 x5 x6 x7)
+    then show ?case apply (cases x7, auto simp add: Rtxn_RegK_Kvtm_Cmt_in_rs_def tps_trans_defs)
       by (metis option.inject)
   next
-    case (RegR x1 x2 x3 x4 x5)
+    case (RegR x1 x2 x3 x4 x5 x6 x7)
     then show ?case 
       apply (auto simp add: Rtxn_RegK_Kvtm_Cmt_in_rs_def tps_trans_defs add_to_readerset_def
                   split: ver_state.split)
       by (metis ver_state.inject(2))
   next
-    case (PrepW x1 x2 x3 x4)
+    case (PrepW x1 x2 x3 x4 x5)
     then show ?case apply (simp add: Rtxn_RegK_Kvtm_Cmt_in_rs_def tps_trans_defs)
       by (metis ver_state.distinct(3))
   next
-    case (CommitW x1 x2 x3 x4 x5)
+    case (CommitW x1 x2 x3 x4 x5 x6 x7)
     then show ?case apply (simp add: Rtxn_RegK_Kvtm_Cmt_in_rs_def tps_trans_defs)
       by (metis ver_state.distinct(5))
   qed (auto simp add: Rtxn_RegK_Kvtm_Cmt_in_rs_def tps_trans_defs)
@@ -2490,7 +2458,7 @@ next
   case (reach_trans s e s')
   then show ?case
   proof (induction e)
-    case (RegR x1 x2 x3 x4 x5)
+    case (RegR x1 x2 x3 x4 x5 x6 x7)
     hence "\<And>k. wtxns_dom (svr_state (svrs s' k)) = wtxns_dom (svr_state (svrs s k))"
       by (simp add: tps_trans_defs add_to_readerset_wtxns_dom)
     hence "\<And>k. wtxns_rsran (svr_state (svrs s' k)) =
@@ -2501,10 +2469,10 @@ next
     then show ?case using RegR apply (simp add: Disjoint_RW_def)
       using Fresh_wr_notin_Wts_dom_def[of s "get_cl x2"] sorry
   next
-    case (PrepW x1 x2 x3 x4)
+    case (PrepW x1 x2 x3 x4 x5)
     then show ?case apply (auto simp add: Disjoint_RW_def tps_trans_defs) sorry
   next
-    case (CommitW x1 x2 x3 x4 x5)
+    case (CommitW x1 x2 x3 x4 x5 x6 x7)
     then show ?case sorry
   qed (auto simp add: Disjoint_RW_def tps_trans_defs)
 qed
@@ -2546,7 +2514,7 @@ next
         sorry
       done
   next
-    case (WCommit x1 x2 x3 x4 x5 x6)
+    case (WCommit x1 x2 x3 x4 x5 x6 x7)
     then show ?case sorry
   qed (auto simp add: Disjoint_RW'_def)
 qed*)
@@ -2569,7 +2537,7 @@ next
     case (RDone x1 x2 x3 x4 x5)
     then show ?case apply (auto simp add: RO_has_rts_def tps_trans_defs) sorry
   next
-    case (WCommit x1 x2 x3 x4 x5 x6)
+    case (WCommit x1 x2 x3 x4 x5 x6 x7)
     then show ?case apply (auto simp add: RO_has_rts_def tps_trans_defs split: if_split_asm) sorry
     (* inv: if t : RO in K it remains RO in K' *)
   qed (auto simp add: RO_has_rts_def tps_trans_defs)
@@ -2612,7 +2580,7 @@ next
   case (reach_trans s e s')
   then show ?case
   proof (induction e)
-    case (WCommit x1 x2 x3 x4 x5 x6)
+    case (WCommit x1 x2 x3 x4 x5 x6 x7)
     then show ?case apply (auto simp add: SO_RO_WR_def tps_trans_defs SO_def SO0_def) sorry
   next
     case (RDone x1 x2 x3 x4 x5)
@@ -2821,12 +2789,12 @@ lemma read_done_ctx_closed:
                                                             
 \<comment> \<open>write_commit closedness (canCommit)\<close>
 lemma write_commit_WR_onK:
-  assumes "write_commit cl kv_map commit_t sn u'' clk s s'"
+  assumes "write_commit cl kv_map commit_t sn u'' clk mmap s s'"
   shows "R_onK WR (kvs_of_s s') = R_onK WR (kvs_of_s s)"
   apply (auto simp add: R_onK_def WR_def) sorry
 
 lemma write_commit_same_rel:
-  assumes "write_commit cl kv_map commit_t sn u'' clk s s'"
+  assumes "write_commit cl kv_map commit_t sn u'' clk mmap s s'"
   shows "R_CC (kvs_of_s s') = R_CC (kvs_of_s s)"
   using assms
   by (auto simp add: R_CC_def write_commit_WR_onK)
@@ -2836,7 +2804,7 @@ lemma "dom kv_map \<noteq> {} \<Longrightarrow> snd ` (\<Union>k\<in>dom kv_map.
   by (metis domIff insertI1 sndI)
 
 lemma write_commit_ctx_closed:    (* HERE *)
-  assumes "write_commit cl kv_map commit_t sn u'' clk s s'"
+  assumes "write_commit cl kv_map commit_t sn u'' clk mmap s s'"
     and "closed' (kvs_of_s s) (cl_ctx (cls s cl)) (R_CC (kvs_of_s s))"
     and "closed_general {get_wtxn s cl} ((R_CC (kvs_of_s s))\<inverse>)
           (visTx' (kvs_of_s s) (cl_ctx (cls s cl)) \<union> read_only_Txs (kvs_of_s s))"
@@ -2895,14 +2863,14 @@ next
   case (reach_trans s e s')
   then show ?case 
   proof (induction e)
-    case (RegR x1 x2 x3 x4 x5)
+    case (RegR x1 x2 x3 x4 x5 x6 x7)
     then show ?case apply (auto simp add: RO_WO_Inv_def tps_trans_defs) sorry
      (*using add_to_readerset_v_writer_img[of ] apply (simp add: txid_defs) sorry \<comment> \<open>Continue here!\<close>*)
   next
-    case (PrepW x1 x2 x3 x4)
+    case (PrepW x1 x2 x3 x4 x5)
     then show ?case sorry
   next
-    case (CommitW x1 x2 x3 x4 x5)
+    case (CommitW x1 x2 x3 x4 x5 x6 x7)
     then show ?case sorry
   qed (auto simp add: RO_WO_Inv_def tps_trans_defs)
 qed
@@ -2929,7 +2897,7 @@ next
     then show ?case apply (simp add: View_Init_def tps_trans_defs get_view_def)
       by (meson Gst_le_Min_Lst_map_def dual_order.trans reach_gst_le_min_lst_map)
   next
-    case (RegR x1 x2 x3 x4 x5)
+    case (RegR x1 x2 x3 x4 x5 x6 x7)
     then show ?case apply (simp add: View_Init_def tps_trans_defs get_view_def)
       using add_to_readerset_no_ver_inv by blast
   qed (auto simp add: View_Init_def tps_trans_defs get_view_def)
@@ -2956,16 +2924,16 @@ next
     case (RInvoke x1 x2 x3 x4)
     then show ?case apply (auto simp add: Get_View_Committed_def tps_trans_defs get_view_def) sorry
   next
-    case (WCommit x1 x2 x3 x4 x5 x6)
+    case (WCommit x1 x2 x3 x4 x5 x6 x7)
     then show ?case apply (auto simp add: Get_View_Committed_def tps_trans_defs get_view_def) sorry
   next
-    case (WDone x1 x2 x3 x4)
+    case (WDone x1 x2 x3 x4 x5)
     then show ?case apply (auto simp add: Get_View_Committed_def tps_trans_defs get_view_def) sorry
   next
-    case (RegR x1 x2 x3 x4 x5)
+    case (RegR x1 x2 x3 x4 x5 x6 x7)
     then show ?case apply (auto simp add: Get_View_Committed_def tps_trans_defs get_view_def) sorry
   next
-    case (PrepW x1 x2 x3 x4)
+    case (PrepW x1 x2 x3 x4 x5)
     then show ?case apply (auto simp add: Get_View_Committed_def tps_trans_defs get_view_def) sorry
   qed (auto simp add: Get_View_Committed_def tps_trans_defs get_view_def)
 qed
@@ -2995,13 +2963,13 @@ next
     then show ?case using read_done_ctx_closed get_ctx_closed
       apply (auto simp add: Deps_Closed_def tps_trans_defs) sorry
   next
-    case (WCommit x1 x2 x3 x4 x5 x6)
+    case (WCommit x1 x2 x3 x4 x5 x6 x7)
     then show ?case apply (simp add: Deps_Closed_def tps_trans_defs) sorry
   next
-    case (RegR x1 x2 x3 x4 x5)
+    case (RegR x1 x2 x3 x4 x5 x6 x7)
     then show ?case sorry
   next
-    case (CommitW x1 x2 x3 x4 x5)
+    case (CommitW x1 x2 x3 x4 x5 x6 x7)
     then show ?case sorry
   qed (auto simp add: Deps_Closed_def tps_trans_defs)
 qed
@@ -3027,11 +2995,11 @@ next
   case (reach_trans s e s')
   then show ?case
   proof (induction e)
-    case (WCommit x1 x2 x3 x4 x5 x6)
+    case (WCommit x1 x2 x3 x4 x5 x6 x7)
     then show ?case apply (simp add: Cl_WtxnCommit_Get_View_def tps_trans_defs get_view_def)
       by (meson domI wtxns_domI1 wtxns_domIff)
   next
-    case (RegR x1 x2 x3 x4 x5)
+    case (RegR x1 x2 x3 x4 x5 x6 x7)
     then show ?case apply (simp add: Cl_WtxnCommit_Get_View_def tps_trans_defs get_view_def)
       by (simp add: add_to_readerset_wtxns_dom)
   qed (auto simp add: Cl_WtxnCommit_Get_View_def tps_trans_defs get_view_def)
@@ -3070,22 +3038,22 @@ next
     case (RInvoke x1 x2 x3 x4)
     then show ?case apply (auto simp add: RegR_Fp_Inv_def tps_trans_defs) sorry
   next
-    case (Read x1 x2 x3 x4 x5 x6 x7 x8)
+    case (Read x1 x2 x3 x4 x5 x6 x7)
     then show ?case apply (auto simp add: RegR_Fp_Inv_def tps_trans_defs) sorry
   next
     case (RDone x1 x2 x3 x4 x5)
     then show ?case apply (auto simp add: RegR_Fp_Inv_def tps_trans_defs) sorry
   next
-    case (WCommit x1 x2 x3 x4 x5 x6)
+    case (WCommit x1 x2 x3 x4 x5 x6 x7)
     then show ?case apply (auto simp add: RegR_Fp_Inv_def tps_trans_defs) sorry
   next
-    case (RegR x1 x2 x3 x4 x5)
+    case (RegR x1 x2 x3 x4 x5 x6 x7)
     then show ?case apply (auto simp add: RegR_Fp_Inv_def tps_trans_defs) sorry
   next
-    case (PrepW x1 x2 x3 x4)
+    case (PrepW x1 x2 x3 x4 x5)
     then show ?case apply (auto simp add: RegR_Fp_Inv_def tps_trans_defs) sorry
   next
-    case (CommitW x1 x2 x3 x4 x5)
+    case (CommitW x1 x2 x3 x4 x5 x6 x7)
     then show ?case apply (auto simp add: RegR_Fp_Inv_def tps_trans_defs) sorry
   qed (auto simp add: RegR_Fp_Inv_def tps_trans_defs get_view_def)
 qed
@@ -3109,22 +3077,22 @@ next
   case (reach_trans s e s')
   then show ?case using kvs_of_s_inv[of s e s']
   proof (induction e)
-    case (Read x1 x2 x3 x4 x5 x6 x7 x8)
+    case (Read x1 x2 x3 x4 x5 x6 x7)
     then show ?case apply (auto simp add: Rtxn_Fp_Inv_def tps_trans_defs) sorry
   next
     case (RDone x1 x2 x3 x4 x5)
     then show ?case sorry
   next
-    case (WCommit x1 x2 x3 x4 x5 x6)
+    case (WCommit x1 x2 x3 x4 x5 x6 x7)
     then show ?case sorry
   next
-    case (RegR x1 x2 x3 x4 x5)
+    case (RegR x1 x2 x3 x4 x5 x6 x7)
     then show ?case sorry
   next
-    case (PrepW x1 x2 x3 x4)
+    case (PrepW x1 x2 x3 x4 x5)
     then show ?case sorry
   next
-    case (CommitW x1 x2 x3 x4 x5)
+    case (CommitW x1 x2 x3 x4 x5 x6 x7)
     then show ?case sorry
   qed (auto simp add: Rtxn_Fp_Inv_def tps_trans_defs view_of_def get_view_def)
 qed
@@ -3151,18 +3119,18 @@ next
     case (RInvoke x1 x2 x3 x4)
     then show ?case sorry
 next
-    case (Read x1 x2 x3 x4 x5 x6 x7 x8)
+    case (Read x1 x2 x3 x4 x5 x6 x7)
     then show ?case apply (auto simp add: Rtxn_notin_rs_other_t_def tps_trans_defs)
       by meson
   next
-    case (RegR x1 x2 x3 x4 x5)
+    case (RegR x1 x2 x3 x4 x5 x6 x7)
     then show ?case apply (auto simp add: Rtxn_notin_rs_other_t_def tps_trans_defs
           split: ver_state.split) sorry
   next
-    case (PrepW x1 x2 x3 x4)
+    case (PrepW x1 x2 x3 x4 x5)
     then show ?case by (simp add: Rtxn_notin_rs_other_t_def tps_trans_defs, blast)
   next
-    case (CommitW x1 x2 x3 x4 x5)
+    case (CommitW x1 x2 x3 x4 x5 x6 x7)
     then show ?case by (simp add: Rtxn_notin_rs_other_t_def tps_trans_defs, blast)
   qed (auto simp add: Rtxn_notin_rs_other_t_def tps_trans_defs)
 qed
@@ -3427,7 +3395,7 @@ lemma set_cts_order_incl_kvs_tids:
 subsubsection \<open>Write commit guard properties\<close>
 
 lemma write_commit_txn_to_vers_get_wtxn:
-  assumes "write_commit cl kv_map cts sn u'' clk gs gs'" 
+  assumes "write_commit cl kv_map commit_t sn u'' clk mmap gs gs'" 
   and "kv_map k = Some v" 
   shows "txn_to_vers gs k (get_wtxn gs cl) = new_vers (Tn (Tn_cl sn cl)) v"
   using assms
@@ -3435,13 +3403,13 @@ lemma write_commit_txn_to_vers_get_wtxn:
       dest!: bspec[where x=k] split: ver_state.split)
 (*
 lemma write_commit_extended_view:    (* NOT USED? *)
-  assumes "write_commit cl kv_map cts sn u'' clk gs gs'" 
+  assumes "write_commit cl kv_map commit_t sn u'' clk mmap gs gs'" 
   shows "u'' = view_of (cts_order gs) (cl_ctx (cls gs cl))"
   using assms
   by (simp add: write_commit_def)
 
 lemma write_commit_seqn:    (* NOT USED? *)
-  assumes "write_commit cl kv_map cts sn u'' clk gs gs'" 
+  assumes "write_commit cl kv_map commit_t sn u'' clk mmap gs gs'" 
   shows "sn = cl_sn (cls gs cl)"
   using assms
   by (simp add: write_commit_def write_commit_G_def)
@@ -3454,21 +3422,21 @@ subsubsection \<open>Write commit update properties\<close>
 
 (*
 lemma write_commit_cl_sn_update:
-  assumes "write_commit cl kv_map cts sn u'' clk gs gs'"
+  assumes "write_commit cl kv_map commit_t sn u'' clk mmap gs gs'"
   shows "cl_sn (cls gs' cl') = cl_sn (cls gs cl')"
   using assms
   by (auto simp add: write_commit_def) 
 *)
 
 lemma write_commit_txn_to_vers_pres:
-  assumes "write_commit_s cl kv_map cts sn u'' clk gs gs'"
+  assumes "write_commit_s cl kv_map cts sn u'' clk mmap gs gs'"
   shows "txn_to_vers gs' k = txn_to_vers gs k"
   using assms
   by (auto 3 4 simp add: tps_trans_defs txn_to_vers_def split: ver_state.split)
 
 
 lemma write_commit_cts_order_update:
-  assumes "write_commit_s cl kv_map cts sn u'' clk gs gs'"
+  assumes "write_commit_s cl kv_map cts sn u'' clk mmap gs gs'"
   shows "cts_order gs' k = 
          (if kv_map k = None
           then cts_order gs k
@@ -3478,7 +3446,7 @@ lemma write_commit_cts_order_update:
 
 
 lemma write_commit_kvs_of_s:
-  assumes "write_commit_s cl kv_map cts sn u'' clk s s'"
+  assumes "write_commit_s cl kv_map cts sn u'' clk mmap s s'"
   shows "kvs_of_s s' = update_kv (Tn_cl sn cl)
                           (write_only_fp kv_map)
                           (view_of (cts_order s) (get_view s cl))
@@ -3494,7 +3462,7 @@ lemma write_commit_kvs_of_s:
 
 NO LONGER HOLDS
 lemma write_commit_views_of_s:
-  assumes "write_commit cl kv_map commit_t sn u'' clk s s'"
+  assumes "write_commit cl kv_map commit_t sn u'' clk mmap s s'"
   shows "views_of_s s' = 
          (\<lambda>cl'. view_of (ext_corder (get_wtxn s cl) kv_map (cts_order s))    
                         (if cl' = cl then insert (get_wtxn s cl) (get_view s cl) 
@@ -3556,7 +3524,7 @@ next
     case (RInvoke x1 x2 x3 x4)
     then show ?case sorry
   next
-    case (Read x1 x2 x3 x4 x5 x6 x7 x8)
+    case (Read x1 x2 x3 x4 x5 x6 x7)
     then show ?case sorry
   next
     case (RDone x1 x2 x3 x4 x5)
@@ -3565,19 +3533,19 @@ next
     case (WInvoke x1 x2 x3 x4)
     then show ?case sorry
   next
-    case (WCommit x1 x2 x3 x4 x5 x6)
+    case (WCommit x1 x2 x3 x4 x5 x6 x7)
     then show ?case sorry
   next
-    case (WDone x1 x2 x3 x4)
+    case (WDone x1 x2 x3 x4 x5)
     then show ?case sorry
   next
-    case (RegR x1 x2 x3 x4 x5)
+    case (RegR x1 x2 x3 x4 x5 x6 x7)
     then show ?case sorry
   next
-    case (PrepW x1 x2 x3 x4)
+    case (PrepW x1 x2 x3 x4 x5)
     then show ?case sorry
   next
-    case (CommitW x1 x2 x3 x4 x5)
+    case (CommitW x1 x2 x3 x4 x5 x6 x7)
     then show ?case sorry
   qed
 qed
@@ -3592,15 +3560,15 @@ proof (induction e)
   case (RInvoke x1 x2 x3 x4)
   then show ?case apply (auto simp add: views_of_s_def tps_trans_defs get_view_def) sorry (* CHECK: does this even hold? *)
 next
-  case (RegR x1 x2 x3 x4 x5)
+  case (RegR x1 x2 x3 x4 x5 x6 x7)
   then show ?case apply (auto simp add: views_of_s_def tps_trans_defs get_view_def
         add_to_readerset_def split: ver_state.split)
     sorry
 next
-  case (PrepW x1 x2 x3 x4)
+  case (PrepW x1 x2 x3 x4 x5)
   then show ?case apply (auto simp add: views_of_s_def tps_trans_defs get_view_def) sorry
 next
-  case (CommitW x1 x2 x3 x4 x5)
+  case (CommitW x1 x2 x3 x4 x5 x6 x7)
   then show ?case apply (auto simp add: views_of_s_def tps_trans_defs get_view_def) sorry
 qed (auto simp add: views_of_s_def tps_trans_defs get_view_def)
 
@@ -3613,7 +3581,7 @@ lemma read_commit_views_of_s_other_cl_inv:
   apply (auto simp add: tps_trans_defs views_of_s_def get_view_def) sorry
 
 lemma write_commit_views_of_s_other_cl_inv:
-  assumes "write_commit_s cl kv_map cts sn u clk s s'"
+  assumes "write_commit_s cl kv_map cts sn u'' clk mmap s s'"
     and "reach tps_s s"
     and "cl' \<noteq> cl"
   shows "views_of_s s' cl' = views_of_s s cl'"
@@ -3639,7 +3607,7 @@ proof (induction e)
     by (auto simp add: tps_trans_defs kvs_expands_def vlist_order_def version_order_def kvs_of_s_defs
         view_atomic_def full_view_def split: ver_state.split)
 next
-  case (WCommit x1 x2 x3 x4 x5 x6)
+  case (WCommit x1 x2 x3 x4 x5 x6 x7)
   then show ?case using t_is_fresh[of s] write_commit_kvs_of_s[of _ x2]
     apply (auto simp add: tps_trans_defs) by (meson kvs_expands_through_update)
 qed auto
@@ -3669,17 +3637,17 @@ next
     then show ?case using RDone
     apply (auto simp add: Views_of_s_Wellformed_def) sorry
   next
-    case (WCommit x1 x2 x3 x4 x5 x6)
+    case (WCommit x1 x2 x3 x4 x5 x6 x7)
     then show ?case
       apply (simp add: Views_of_s_Wellformed_def tps_trans_defs views_of_s_def get_view_def) sorry
   next
-    case (RegR x1 x2 x3 x4 x5)
+    case (RegR x1 x2 x3 x4 x5 x6 x7)
     then show ?case apply (auto simp add: Views_of_s_Wellformed_def tps_trans_defs
           add_to_readerset_def split: ver_state.split) sorry
   next
-    case (PrepW x1 x2 x3 x4)    then show ?case apply (auto simp add: Views_of_s_Wellformed_def tps_trans_defs views_of_s_def get_view_def) sorry
+    case (PrepW x1 x2 x3 x4 x5)    then show ?case apply (auto simp add: Views_of_s_Wellformed_def tps_trans_defs views_of_s_def get_view_def) sorry
   next
-    case (CommitW x1 x2 x3 x4 x5)
+    case (CommitW x1 x2 x3 x4 x5 x6 x7)
     then show ?case apply (auto simp add: Views_of_s_Wellformed_def tps_trans_defs views_of_s_def get_view_def) sorry
   qed (auto simp add: Views_of_s_Wellformed_def tps_trans_defs views_of_s_def get_view_def)
 qed
@@ -3779,11 +3747,11 @@ next
         by (auto simp only: ET_CC.trans_ET_ES_eq tps_trans state_trans.simps sim_def med.simps)
     qed
   next
-    case (WCommit cl kv_map cts sn u'' clk)
+    case (WCommit cl kv_map cts sn u'' clk mmap)
     then show ?case
     proof -
       {
-        assume cmt: \<open>write_commit_s cl kv_map cts sn u'' clk gs gs'\<close>
+        assume cmt: \<open>write_commit_s cl kv_map cts sn u'' clk mmap gs gs'\<close>
         have \<open>ET_CC.ET_trans_and_fp 
                 (kvs_of_s gs, views_of_s gs)
                  (ET cl sn u'' (write_only_fp kv_map))
